ghost references and their use in DisposableInvariant

ulib/experimental/Steel.DisposableInvariant.fst
@@ -6,78 +6,18 @@ module A = Steel.Effect.Atomic
 #push-options "--ide_id_info_off"
 open Steel.Reference
 open FStar.Ghost
-let ghostref (a:Type) = ref (erased a)
-
-let ghost_pts_to (#a:Type) (r:ghostref a) ([@@@smt_fallback]p:perm) ([@@@smt_fallback]x:erased a) =
-  pts_to #(erased a) r p (hide x)
-
-assume
-val alloc_ghost (#a:Type) (#u:_) (x:erased a)
-  : SteelAtomicT (ghostref a) u unobservable
-    emp
-    (fun r -> ghost_pts_to r full_perm x)
-
-
-assume
-val split_ghost (#a:Type) (#u:_)
-                (#p:perm)
-                (#x:erased a)
-                (r:ghostref a)
-  : SteelAtomicT unit u unobservable
-    (ghost_pts_to r p x)
-    (fun _ -> ghost_pts_to r (half_perm p) x `star`
-           ghost_pts_to r (half_perm p) x)
-
-assume
-val gather_ghost (#a:Type) (#u:_)
-                 (#p0 #p1:perm)
-                 (#x0 #x1:erased a)
-                 (r:ghostref a)
-  : SteelAtomic unit u unobservable
-    (ghost_pts_to r p0 x0 `star`
-     ghost_pts_to r p1 x1)
-    (fun _ -> ghost_pts_to r (sum_perm p0 p1) x0)
-    (requires fun _ -> true)
-    (ensures fun _ _ _ -> x0 == x1)
-
-assume
-val pts_to_injective_eq (#a:_) (#u:_) (#p #q:_) (r:ghostref a) (v0 v1:Ghost.erased a)
-  : SteelAtomic unit u unobservable (ghost_pts_to r p v0 `star` ghost_pts_to r q v1)
-                     (fun _ -> ghost_pts_to r p v0 `star` ghost_pts_to r q v0)
-                (requires fun _ -> True)
-                (ensures fun _ _ _ -> v0 == v1)
-
-assume
-val write_ghost (#a:Type) (#u:_) (#x:erased a) (r:ghostref a) (v:erased a)
-  : SteelAtomicT unit u unobservable
-    (ghost_pts_to r full_perm x)
-    (fun _ -> ghost_pts_to r full_perm v)
-
-assume
-val admit_atomic (#a:_) (#u:_)
-                 (#[@@@framing_implicit] p:pre_t)
-                 (#[@@@framing_implicit] q:post_t a)
-                 (_:unit)
-  : SteelAtomicF a u unobservable p q (fun _ -> True) (fun _ _ _ -> True)
-
-assume
-val drop (#u:_) (p:slprop)
-  : SteelAtomicT unit u unobservable p (fun _ -> emp)
-
-assume Obs: (observable =!= unobservable)
-
 
 [@@__reduce__]
-let conditional_inv (r:ghostref bool) (p:slprop) =
+let conditional_inv (r:ghost_ref bool) (p:slprop) =
       (fun (b:bool) ->
          ghost_pts_to r (half_perm full_perm) (hide b) `star`
          (if b then p else emp))
 
 [@@__reduce__]
-let ex_conditional_inv (r:ghostref bool) (p:slprop) =
+let ex_conditional_inv (r:ghost_ref bool) (p:slprop) =
     h_exists (conditional_inv r p)
 
-let inv (p:slprop) = (r:ghostref bool & Steel.Memory.inv (ex_conditional_inv r p))
+let inv (p:slprop) = (r:ghost_ref bool & Steel.Memory.inv (ex_conditional_inv r p))
 
 let name (#p:_) (i:inv p) = dsnd i
 let gref (#p:_) (i:inv p) = dfst i
@@ -89,9 +29,9 @@ let active (#p:_) ([@@@smt_fallback]f:perm) (i:inv p) =
 
 let new_inv (#u:_) (p:slprop)
   : SteelAtomicT (inv p) u unobservable p (active full_perm)
-  = let r = alloc_ghost (Ghost.hide true) in
-    split_ghost r;
-    A.intro_h_exists true (conditional_inv r p);
+  = let r = ghost_alloc (Ghost.hide true) in
+    ghost_share r;
+    A.intro_exists true (conditional_inv r p);
     let i = A.new_invariant u (ex_conditional_inv r p) in
     (| r, i |)
 
@@ -99,26 +39,23 @@ let share (#p:slprop) (#f:perm) (#u:_) (i:inv p)
   : SteelAtomicT unit u unobservable
     (active f i)
     (fun _ -> active (half_perm f) i `star` active (half_perm f) i)
-  = split_ghost (gref i)
+  = ghost_share (gref i)
 
 let gather (#p:slprop) (#f0 #f1:perm) (#u:_) (i:inv p)
   : SteelAtomicT unit u unobservable
     (active f0 i `star` active f1 i)
     (fun _ -> active (sum_perm f0 f1) i)
-  = gather_ghost #_ #_ #(half_perm f0) (gref i);
+  = ghost_gather #_ #_ #(half_perm f0) (gref i);
     A.change_slprop
       (ghost_pts_to (gref i) (sum_perm (half_perm f0) (half_perm f1)) (hide true))
       (ghost_pts_to (gref i) (half_perm (sum_perm f0 f1)) (hide true))
       (fun _ -> assert (FStar.Real.two == 2.0R); assert (sum_perm (half_perm f0) (half_perm f1) == (half_perm (sum_perm f0 f1))))
 
-
-let iinv (#p:_) (i:inv p) : Steel.Memory.inv (ex_conditional_inv (gref i) p) = name i
-
 let dispose (#p:slprop) (#u:_) (i:inv p{not (name i `Set.mem` u)})
   : SteelAtomicT unit u unobservable
     (active full_perm i)
     (fun _ -> p)
-  = let dispose_aux (r:ghostref bool) (_:unit)
+  = let dispose_aux (r:ghost_ref bool) (_:unit)
     : SteelAtomicT unit (set_add (name i) u)  unobservable
        (ex_conditional_inv r p `star`
         ghost_pts_to r (half_perm full_perm) true)
@@ -126,17 +63,17 @@ let dispose (#p:slprop) (#u:_) (i:inv p{not (name i `Set.mem` u)})
         ex_conditional_inv r p `star`
         p)
     = let b = A.witness_h_exists #_ #_ #(conditional_inv r p) () in
-      gather_ghost #_ #_ #_ #_ #true #(hide (reveal b)) r;
+      ghost_gather #_ #_ #_ #_ #true #(hide (reveal b)) r;
       A.change_slprop (if b then p else emp) p (fun _ -> ());
       A.change_slprop (ghost_pts_to r (sum_perm (half_perm full_perm) (half_perm full_perm)) true)
                       (ghost_pts_to r full_perm true)
                       (fun _ -> ());
-      write_ghost r false;
-      split_ghost r;
-      A.intro_h_exists false (conditional_inv r p);
+      ghost_write r false;
+      ghost_share r;
+      A.intro_exists false (conditional_inv r p);
       drop (ghost_pts_to r (half_perm full_perm) false)
     in
-    A.with_invariant (iinv i)
+    A.with_invariant (name i)
                      (dispose_aux (gref i))
 
 let with_invariant (#a:Type)
@@ -151,7 +88,7 @@ let with_invariant (#a:Type)
                                              (p `star` fp)
                                              (fun x -> p `star` fp' x))
   : SteelAtomicT a u o (active perm i `star` fp) (fun x -> active perm i `star` fp' x)
-  = let with_invariant_aux (r:ghostref bool)
+  = let with_invariant_aux (r:ghost_ref bool)
                            (_:unit)
       : SteelAtomicT a (set_add (name i) u) o
           (ex_conditional_inv r p `star`
@@ -162,11 +99,11 @@ let with_invariant (#a:Type)
           (ghost_pts_to r (half_perm perm) true `star` //associativity matters
           fp' x))
     = let b = A.witness_h_exists #_ #_ #(conditional_inv r p) () in
-      pts_to_injective_eq r true (hide (reveal b));
+      ghost_pts_to_injective_eq r true (hide (reveal b));
       A.change_slprop (if b then p else emp) p (fun _ -> ());
       let x = f() in
-      A.intro_h_exists true (conditional_inv r p);
+      A.intro_exists true (conditional_inv r p);
       x
     in
-    A.with_invariant (iinv i)
+    A.with_invariant (name i)
                      (with_invariant_aux (gref i))
